poSTVM/poSTVM_alt_inductive.thy
@@ -2,7 +2,7 @@ theory poSTVM_alt_inductive
   imports 
     "~~/poST/poSTVM/poSTVM_state_alt" 
 begin
-datatype statement_result =  Continue | Exit | Return | Reset
+datatype statement_result =  Continue | Exit | Return 
 
 
 
@@ -99,7 +99,7 @@ inductive
                         None \<Rightarrow> (statement_result.Continue, set_next_state_next (snd st))
                       | Some name \<Rightarrow> (statement_result.Continue, set_state (snd st) name))\<rbrakk>\<Longrightarrow>
                 st\<turnstile>stmt.SetStateSt st_name_option\<longrightarrow>st1"
-  | Reset : "st\<turnstile>stmt.ResetSt\<longrightarrow>(statement_result.Reset, snd st)"
+  | Reset : "st\<turnstile>stmt.ResetSt\<longrightarrow>(statement_result.Continue,reset_timer( snd st))"
 
 print_theorems
 (*
@@ -136,10 +136,8 @@ inductive eval_state :: "[model_state,stacked_state,statement_result * model_sta
                   | (_) \<Rightarrow> (res,st2) = (res,st1))\<rbrakk> \<Longrightarrow> 
                 st \<turnstile>(name,looped,stm,timeout_op):(res,st2)"
 
-
-
-(*TO DO RESET*)
-inductive eval_process :: "[model_state,stacked_process,model_state] \<Rightarrow> bool" ("_\<turnstile>_\<Rightarrow>_") where
+inductive eval_process :: "[model_state,stacked_process,model_state] \<Rightarrow> bool" ("_\<turnstile>_\<Rightarrow>_") and
+          evals_process :: "[model_state,stacked_process list,model_state] \<Rightarrow> bool" ("_\<turnstile>_[\<Rightarrow>]_") where
     ProcStep : "\<lbrakk> new_st = (set_cur_proc_name st name);
                   new_st\<turnstile>(get_state_by_name state_list (get_cur_proc_state_name new_st)) :(res,st1);
                   st2 = (case res of 
@@ -148,16 +146,26 @@ inductive eval_process :: "[model_state,stacked_process,model_state] \<Rightarro
                         | statement_result.Return \<Rightarrow> st1);
                   st3 = (process_vars_distribution (set_into_next_state st2))\<rbrakk> \<Longrightarrow> 
                 st\<turnstile>(name,var_list,state_list) \<Rightarrow> st3"
+  | ProcNil : "st\<turnstile>[][\<Rightarrow>]st"
+  | ProcCons : "\<lbrakk>st\<turnstile>pr\<Rightarrow>st1;
+                 (process_vars_distribution st1)\<turnstile>other[\<Rightarrow>]st2 \<rbrakk> \<Longrightarrow> 
+                st\<turnstile>(pr#other)[\<Rightarrow>]st2"
 
 
-(*
-(*add var distribution*)
-inductive eval_program :: "[model_state,stacked_program,model_state] \<Rightarrow> bool" ("_\<turnstile>_\<Longrightarrow>_") where
-    ProgStep : "\<lbrakk>new_st = (set_cur_prog_name st name); 
-                  st2 = (foldl (\<lambda>proc st1. st1 ) new_st process_list)\<rbrakk>\<Longrightarrow> 
-              st\<turnstile>(name,var_list,process_list) \<Longrightarrow>st2"
-*)
+inductive eval_program :: "[model_state,stacked_program,model_state] \<Rightarrow> bool" ("_\<turnstile>_\<Longrightarrow>_") and
+          eval_programs :: "[model_state,stacked_program list,model_state] \<Rightarrow> bool" ("_\<turnstile>_[\<Longrightarrow>]_") where
+    ProgStep : "\<lbrakk>new_st = (set_cur_prog_name st name);
+                 new_st\<turnstile>(filter_active_processes new_st process_list)[\<Rightarrow>]st1\<rbrakk>\<Longrightarrow> 
+              st\<turnstile>(name,var_list,process_list) \<Longrightarrow>st1"
+  | ProgNil : "st\<turnstile>[][\<Longrightarrow>]st"
+  | ProgCons : "\<lbrakk>st\<turnstile>pr\<Longrightarrow>st1;
+                 (process_vars_distribution st1)\<turnstile>other[\<Longrightarrow>]st2\<rbrakk> \<Longrightarrow> 
+               st\<turnstile>(pr#other)[\<Longrightarrow>]st2"
 
+
+inductive eval_model :: "[model_state,stacked_model,model_state] \<Rightarrow> bool" ("_\<turnstile>_\<mapsto>_") where
+    ModelStep : "\<lbrakk>st\<turnstile>prog_list[\<Longrightarrow>]st1\<rbrakk> \<Longrightarrow>
+                st\<turnstile>(_,_,prog_list,_,_)\<mapsto>st1"
 
 (*
 apply (simp add: const_to_basic_def
